Correctness of pack

frodo/code/Hacl.Impl.Frodo.Pack.fst
@@ -18,7 +18,120 @@ module ST = FStar.HyperStack.ST
 module Lemmas = Spec.Frodo.Lemmas
 module S = Spec.Frodo.Pack
 
-#reset-options "--z3rlimit 50 --max_fuel 0 --max_ifuel 0 --using_facts_from '* -Spec'"
+#reset-options "--z3rlimit 50 --max_fuel 0 --max_ifuel 0 --using_facts_from '* -Spec +Spec.Frodo.Pack'"
+
+module Seq = Lib.Sequence
+
+inline_for_extraction noextract
+val frodo_pack8:
+    a:lbuffer uint16 8
+  -> d:size_t{v d <= 16}
+  -> res:lbytes d
+  -> Stack unit
+    (requires fun h0 -> live h0 a /\ live h0 res /\ disjoint a res)
+    (ensures  fun h0 _ h1 -> modifies (loc_buffer res) h0 h1 /\
+      as_seq h1 res == S.frodo_pack8 (as_seq h0 a) (v d))
+let frodo_pack8 a d res =
+  let h0 = ST.get() in
+  push_frame();
+  let maskd = to_u16 (u32 1 <<. size_to_uint32 d) -. u16 1 in
+  let v16 = create #_ #16 (size 16) (u8 0) in
+  let a0 = index a (size 0) &. maskd in
+  let a1 = index a (size 1) &. maskd in
+  let a2 = index a (size 2) &. maskd in
+  let a3 = index a (size 3) &. maskd in
+  let a4 = index a (size 4) &. maskd in
+  let a5 = index a (size 5) &. maskd in
+  let a6 = index a (size 6) &. maskd in
+  let a7 = index a (size 7) &. maskd in
+  let templong =
+       to_u128 a0 <<. size_to_uint32 (size 7 *! d)
+    |. to_u128 a1 <<. size_to_uint32 (size 6 *! d)
+    |. to_u128 a2 <<. size_to_uint32 (size 5 *! d)
+    |. to_u128 a3 <<. size_to_uint32 (size 4 *! d)
+    |. to_u128 a4 <<. size_to_uint32 (size 3 *! d)
+    |. to_u128 a5 <<. size_to_uint32 (size 2 *! d)
+    |. to_u128 a6 <<. size_to_uint32 (size 1 *! d)
+    |. to_u128 a7 <<. size_to_uint32 (size 0 *! d)
+  in
+  uint_to_bytes_be v16 templong;
+  let src = sub v16 (size 16 -! d) d in // Skips the 1st byte when d = 15
+  copy res d src;
+  pop_frame()
+
+inline_for_extraction noextract
+val frodo_pack8':
+    #n1:size_t
+  -> #n2:size_t{v n1 * v n2 <= max_size_t /\ v n2 % 8 = 0}
+  -> a8:lbuffer uint16 8
+  -> d:size_t{v d * (v n1 * v n2 / 8) <= max_size_t /\ v d <= 16}
+  -> res:lbytes (d *! (n1 *! n2 /. size 8))
+  -> i:size_t{v i < v n1 * v n2 / 8}
+  -> Stack unit
+    (requires fun h0 -> live h0 a8 /\ live h0 res /\ disjoint a8 res)
+    (ensures  fun h0 _ h1 ->
+      modifies (loc_buffer res) h0 h1 /\
+      Seq.equal
+        (as_seq h1 (gsub #_ #_ #(v d) res (d *! i) d))
+        (S.frodo_pack8 (as_seq h0 a8) (v d)) /\
+      (forall (j:nat{j < v i}).
+        {:pattern as_seq h1 (gsub #_ #_ #(v d) res (d *! size j) d)}
+        v d * j + v d <= v d * (v n1 * v n2 / 8) /\
+        Seq.equal #_ #(v d)
+          (as_seq h1 (gsub #_ #_ #(v d) res (d *! size j) d))
+          (as_seq h0 (gsub #_ #_ #(v d) res (d *! size j) d))))
+let frodo_pack8' #n1 #n2 a8 d res i =
+  let r = sub #_ #_ #(v d) res (d *! i) d in
+  frodo_pack8 a8 d r
+
+val frodo_pack:
+    #n1:size_t
+  -> #n2:size_t{v n1 * v n2 <= max_size_t /\ v n2 % 8 = 0}
+  -> a:matrix_t n1 n2
+  -> d:size_t{v d * (v n1 * v n2 / 8) <= max_size_t /\ v d <= 16}
+  -> res:lbytes (d *! (n1 *! n2 /. size 8))
+  -> Stack unit
+    (requires fun h -> live h a /\ live h res /\ disjoint a res /\
+      0 < v d /\ 0 < v n1 * v n2 / 8)
+    (ensures  fun h0 _ h1 ->
+      modifies (loc_buffer res) h0 h1 /\
+      as_seq h1 res == S.frodo_pack (as_matrix h0 a) (v d))
+[@"c_inline"]
+let frodo_pack #n1 #n2 a d res =
+  let h0 = ST.get () in
+  assert (forall (j:nat{j < v n1 * v n2 / 8}). v d * j + v d <= v d * (v n1 * v n2 / 8));
+  let inv h (i:nat{i <= v n1 * v n2 / 8}) =
+    modifies (loc_buffer res) h0 h /\
+    (forall (j:nat{j < i}).//{:pattern as_seq h1 (gsub #_ #_ #(v d) res (d *! size j) d)}
+      let a8 = Seq.sub #uint16 (as_matrix h0 a) (8 * j) 8 in
+      Seq.equal
+        (as_seq h (gsub #_ #_ #(v d) res (d *! size j) d))
+        (S.frodo_pack8 a8 (v d)))
+  in
+  let f (i:size_t{v i < v n1 * v n2 / 8}) : Stack unit
+    (requires fun h1 -> inv h1 (v i))
+    (ensures  fun _ _ h2 -> inv h2 (v i + 1)) =
+      let a8 = sub a (size 8 *! i) (size 8) in
+      frodo_pack8' a8 d res i
+  in
+  Lib.Loops.for (size 0) (n1 *! n2 /. size 8) inv f;
+  let h1 = ST.get() in
+  let a0 = as_matrix h0 a in
+  let res0 = S.frodo_pack a0 (v d) in
+  let f (j:nat{j < v n1 * v n2 / 8}) : Lemma
+    (let a8 = Seq.sub #uint16 a0 (8 * j) 8 in
+     Seq.equal
+       (as_seq h1 (gsub #_ #_ #(v d) res (d *! size j) d))
+       (Seq.sub res0 (v d * j) (v d)))
+  = 
+    let a8 = Seq.sub #uint16 a0 (8 * j) 8 in
+    Seq.eq_elim (Seq.sub res0 (v d * j) (v d)) (S.frodo_pack8 a8 (v d))
+  in
+  Classical.forall_intro f;
+  S.bar (v n1 * v n2 / 8) (v d) (as_seq h1 res) (S.frodo_pack a0 (v d))
+
+
+/// Unpack
 
 private
 val shift_left_bounds: d:size_nat{d <= 16} ->
@@ -32,105 +145,6 @@ val shift_left_bounds: d:size_nat{d <= 16} ->
     1 * d < bits U128 /\
     0 * d < bits U128)
 let shift_left_bounds d = ()
-
-private
-let modifies_popped (#a:Type) (b1:buffer a) (b2:buffer a) (h0:mem) h1 (h2:mem) h3 :
-  Lemma
-    (requires
-      live h0 b1 /\
-      fresh_frame h0 h1 /\
-      modifies (loc_union (loc_buffer b1) (loc_buffer b2)) h1 h2 /\
-      get_tip h2 == get_tip h1 /\
-      popped h2 h3)
-    (ensures live h3 b1)
-  [SMTPat (fresh_frame h0 h1); SMTPat (popped h2 h3); SMTPat (live h0 b1);
-   SMTPat (modifies (loc_union (loc_buffer b1) (loc_buffer b2)) h1 h2)]
-= ()
-
-
-inline_for_extraction noextract
-val frodo_pack_inner:
-    #n1:size_t
-  -> #n2:size_t{v n1 * v n2 <= max_size_t /\ v n2 % 8 = 0}
-  -> a:matrix_t n1 n2
-  -> d:size_t{v d * v n1 <= max_size_t /\ v d * v n1 * v n2 <= max_size_t /\ v d <= 16}
-  -> res:lbytes (d *! n1 *! n2 /. size 8)
-  -> i:size_t{v i < v n1}
-  -> Stack unit
-    (requires fun h -> live h a /\ live h res /\ disjoint a res)
-    (ensures  fun h0 _ h1 -> live h1 res /\ modifies (loc_buffer res) h0 h1)
-let frodo_pack_inner #n1 #n2 a d res i =
-  shift_left_bounds (v d);
-  push_frame();
-  let maskd = to_u16 (u32 1 <<. size_to_uint32 d) -. u16 1 in
-  let v16 = create #_ #16 (size 16) (u8 0) in
-  let n28 = n2 /. size 8 in
-  let h0 = ST.get () in
-  let inv h1 (j:nat{j <= v n28}) =
-    live h1 res /\
-    live h1 v16 /\
-    modifies (loc_union (loc_buffer res) (loc_buffer v16)) h0 h1
-  in
-  let f (j:size_t{v j < v n28}) : Stack unit
-    (requires fun h -> inv h (v j))
-    (ensures  fun _ _ h2 -> inv h2 (v j + 1)) =
-      Lemmas.lemma_matrix_index_repeati (v n1) (v n2) (v d) (v i) (v j);
-      let start = (i *! n28 +! j) *! d in
-      assert_spinoff (v start + v d <= v d * v n1 * v n2 / 8);
-      let aij0 = a.[i, size 8 *! j +! size 0] &. maskd in
-      let aij1 = a.[i, size 8 *! j +! size 1] &. maskd in
-      let aij2 = a.[i, size 8 *! j +! size 2] &. maskd in
-      let aij3 = a.[i, size 8 *! j +! size 3] &. maskd in
-      let aij4 = a.[i, size 8 *! j +! size 4] &. maskd in
-      let aij5 = a.[i, size 8 *! j +! size 5] &. maskd in
-      let aij6 = a.[i, size 8 *! j +! size 6] &. maskd in
-      let aij7 = a.[i, size 8 *! j +! size 7] &. maskd in
-      let templong =
-           to_u128 aij0 <<. size_to_uint32 (size 7 *! d)
-        |. to_u128 aij1 <<. size_to_uint32 (size 6 *! d)
-        |. to_u128 aij2 <<. size_to_uint32 (size 5 *! d)
-        |. to_u128 aij3 <<. size_to_uint32 (size 4 *! d)
-        |. to_u128 aij4 <<. size_to_uint32 (size 3 *! d)
-        |. to_u128 aij5 <<. size_to_uint32 (size 2 *! d)
-        |. to_u128 aij6 <<. size_to_uint32 (size 1 *! d)
-        |. to_u128 aij7 <<. size_to_uint32 (size 0 *! d)
-      in
-      uint_to_bytes_be v16 templong;
-      let src = sub v16 (size 16 -! d) d in // Skips the 1st byte when d = 15
-      update_sub res start d src
-  in
-  Lib.Loops.for (size 0) n28 inv f;
-  pop_frame()
-
-
-val frodo_pack:
-    #n1:size_t
-  -> #n2:size_t{v n1 * v n2 <= max_size_t /\ v n2 % 8 = 0}
-  -> a:matrix_t n1 n2
-  -> d:size_t{v d * v n1 <= max_size_t /\ v d * v n1 * v n2 <= max_size_t /\ v d <= 16}
-  -> res:lbytes (d *! n1 *! n2 /. size 8)
-  -> Stack unit
-    (requires fun h -> live h a /\ live h res /\ disjoint a res)
-    (ensures  fun h0 _ h1 ->
-      live h1 res /\
-      modifies (loc_buffer res) h0 h1 /\
-      as_seq h1 res == S.frodo_pack (as_matrix h0 a) (v d))
-[@"c_inline"]
-let frodo_pack #n1 #n2 a d res =
-  let h = ST.get () in
-  push_frame();
-  let h0 = ST.get () in
-  let inv h1 (i:nat{i <= v n1}) =
-    live h1 res /\
-    modifies (loc_buffer res) h0 h1
-  in
-  Lib.Loops.for (size 0) n1 inv (frodo_pack_inner a d res);
-  pop_frame();
-  let h' = ST.get() in
-  assume (as_seq h' res == S.frodo_pack (as_matrix h a) (v d))
-
-
-/// Unpack
 
 inline_for_extraction noextract
 val frodo_unpack_inner:
